Symmetry.v
@@ -1,6 +1,5 @@
 Require Import SessionTypes.
 Require Import Equivalence.
-Import Eq Sty.
 
 Inductive sym {A} (R : A -> A -> Prop) : A -> A -> Prop :=
 | sym_sym : forall x y, R x y -> sym R y x
