Transitivity.v
@@ -1,0 +1,11 @@
+Require Import Equivalence SessionTypes Wellformed.
+
+Theorem sequiv_transitive :
+  forall S T U,
+  wellformed S ->
+  wellformed T ->
+  wellformed U ->
+  sequiv S T ->
+  sequiv T U ->
+  sequiv S U.
+Proof. Admitted.
